Make [reflect] a typeclass and add a bunch of lemmas

src/Util/Bool/Reflect.v
@@ -1,5 +1,18 @@
 (** * Some lemmas about [Bool.reflect] *)
+Require Import Coq.Classes.CMorphisms.
 Require Import Coq.Bool.Bool.
+Require Import Coq.Arith.Arith.
+Require Import Coq.ZArith.BinInt Coq.ZArith.ZArith_dec.
+Require Import Coq.NArith.BinNat.
+Require Import Crypto.Util.HProp.
+Require Import Crypto.Util.Decidable.
+Require Import Crypto.Util.Prod.
+Require Import Crypto.Util.Option.
+Require Import Crypto.Util.Sigma.
+Require Import Crypto.Util.ListUtil.
+Require Import Crypto.Util.Sum.
+Require Import Crypto.Util.Comparison.
+Require Import Crypto.Util.Tactics.DestructHead.
 
 Lemma reflect_to_dec_iff {P b1 b2} : reflect P b1 -> (b1 = b2) <-> (if b2 then P else ~P).
 Proof.
@@ -12,13 +25,30 @@ Proof. intro; apply reflect_to_dec_iff; assumption. Qed.
 Lemma reflect_of_dec {P} {b1 b2 : bool} : reflect P b1 -> (if b2 then P else ~P) -> (b1 = b2).
 Proof. intro; apply reflect_to_dec_iff; assumption. Qed.
 
+Lemma reflect_of_brel {A R Rb} (bl : forall a a' : A, Rb a a' = true -> (R a a' : Prop))
+      (lb : forall a a' : A, R a a' -> Rb a a' = true)
+  : forall x y, reflect (R x y) (Rb x y).
+Proof.
+  intros x y; specialize (bl x y); specialize (lb x y).
+  destruct (Rb x y); constructor; intuition congruence.
+Qed.
+
+Lemma reflect_to_brel {A R Rb} (H : forall x y : A, reflect (R x y) (Rb x y))
+  : (forall a a' : A, Rb a a' = true -> R a a')
+    /\ (forall a a' : A, R a a' -> Rb a a' = true).
+Proof.
+  split; intros x y; specialize (H x y); destruct H; intuition congruence.
+Qed.
+
 Lemma reflect_of_beq {A beq} (bl : forall a a' : A, beq a a' = true -> a = a')
       (lb : forall a a' : A, a = a' -> beq a a' = true)
   : forall x y, reflect (x = y) (beq x y).
-Proof.
-  intros x y; specialize (bl x y); specialize (lb x y).
-  destruct (beq x y); constructor; intuition congruence.
-Qed.
+Proof. apply reflect_of_brel; assumption. Qed.
+
+Lemma reflect_to_beq {A beq} (H : forall x y : A, reflect (x = y) (beq x y))
+  : (forall a a' : A, beq a a' = true -> a = a')
+    /\ (forall a a' : A, a = a' -> beq a a' = true).
+Proof. apply reflect_to_brel; assumption. Qed.
 
 Definition mark {T} (v : T) := v.
 
@@ -35,3 +65,207 @@ Ltac beq_to_eq beq bl lb :=
               intros; cbv beta delta [mark]
          | [ H : context[beq ?x ?x] |- _ ] => rewrite (lb x x eq_refl) in H
          end.
+
+Existing Class reflect.
+Definition decb (P : Prop) {b : bool} {H : reflect P b} := b.
+Notation reflect_rel P b := (forall x y, reflect (P x y) (b x y)).
+
+Lemma decb_true_iff P {b} {H : reflect P b} : @decb P b H = true <-> P.
+Proof. symmetry; apply reflect_iff, H. Qed.
+Lemma decb_bp P {b} {H : reflect P b} : @decb P b H = true -> P.
+Proof. apply decb_true_iff. Qed.
+Lemma decb_pb P {b} {H : reflect P b} : P -> @decb P b H = true.
+Proof. apply decb_true_iff. Qed.
+Lemma decb_false_iff P {b} {H : reflect P b} : @decb P b H = false <-> ~P.
+Proof. generalize (decb P), (decb_true_iff P); clear; intros []; intros; intuition congruence. Qed.
+Lemma decb_false_bp P {b} {H : reflect P b} : @decb P b H = false -> ~P.
+Proof. apply decb_false_iff. Qed.
+Lemma decb_false_pb P {b} {H : reflect P b} : ~P -> @decb P b H = false.
+Proof. apply decb_false_iff. Qed.
+
+Global Instance dec_of_reflect P {b} {H : reflect P b} : Decidable P | 15
+  := (if b as b return reflect P b -> Decidable P
+      then fun H => left (decb_bp P eq_refl)
+      else fun H => right (decb_false_bp P eq_refl)) H.
+
+Global Instance eq_decb_hprop {A} {x y : A} {hp : IsHProp A} : reflect (@eq A x y) true | 5.
+Proof. left; auto. Qed.
+
+Ltac solve_reflect_step :=
+  first [ match goal with
+          | [ H : reflect _ ?b |- _ ] => tryif is_var b then destruct H else (inversion H; clear H)
+          | [ |- reflect _ _ ] => constructor
+          | [ |- reflect (?R ?x ?y) (?Rb ?x ?y) ] => apply (@reflect_of_brel _ R Rb)
+          | [ H : forall x y, reflect (?R x y) (?Rb x y) |- _ ] => apply (@reflect_to_brel _ R Rb) in H
+          end
+        | progress destruct_head'_and
+        | progress intros
+        | progress subst
+        | solve [ eauto
+                | firstorder (auto; try discriminate) ]
+            (*
+          | [ H :
+          | [ H : forall x y : ?A, reflect (x = y) _, x0 : ?A, y0 : ?A  |- _ ]
+            => no_equalities_about x0 y0; let H' := fresh in pose proof (H x0 y0) as H'; inversion H'; clear H'
+          | [ H : forall a0 (x y : _), reflect (x = y) _, x0 : ?A, y0 : ?A  |- _ ]
+            => no_equalities_about x0 y0; let H' := fresh in pose proof (H _ x0 y0) as H'; inversion H'; clear H'
+          | [ H : true = ?x |- context[?x] ] => rewrite <- H
+          | [ H : false = ?x |- context[?x] ] => rewrite <- H
+          end
+        | progress intros
+        | split
+        | progress inversion_sigma
+        | progress inversion_prod
+        | progress pre_decide_destruct_sigma
+        | progress destruct_head'_bool
+        | progress destruct_head'_prod
+        | progress subst
+        | progress cbn in *
+        | progress hnf
+        | progress pre_hprop
+        | solve [ left; firstorder (auto; try discriminate)
+                | right; firstorder (auto; try discriminate)
+                | firstorder (auto; try discriminate) ] *) ].
+
+
+Ltac solve_reflect := repeat solve_reflect_step.
+
+Hint Constructors reflect : typeclass_instances.
+
+Local Hint Resolve -> Bool.eqb_true_iff : core.
+Local Hint Resolve <- Bool.eqb_true_iff : core.
+Local Hint Resolve internal_prod_dec_bl internal_prod_dec_lb
+      internal_option_dec_bl internal_option_dec_lb
+      internal_list_dec_bl internal_list_dec_lb
+      internal_sum_dec_bl internal_sum_dec_lb
+      sigT_dec_bl sigT_dec_lb
+      sigT_dec_bl_hprop sigT_dec_lb_hprop
+      sig_dec_bl sig_dec_lb
+      sig_dec_bl_hprop sig_dec_lb_hprop
+      internal_comparison_dec_bl internal_comparison_dec_lb
+  : core.
+
+Local Hint Extern 0 => solve [ solve_reflect ] : typeclass_instances.
+Local Hint Extern 1 => progress inversion_sigma : core.
+
+Global Instance reflect_True : reflect True true | 10 := ReflectT _ I.
+Global Instance reflect_False : reflect False false | 10 := ReflectF _ (fun x => x).
+Global Instance reflect_or {A B a b} `{reflect A a, reflect B b} : reflect (A \/ B) (orb a b) | 10. exact _. Qed.
+Global Instance reflect_and {A B a b} `{reflect A a, reflect B b} : reflect (A /\ B) (andb a b) | 10. exact _. Qed.
+Global Instance reflect_impl_or {A B bona} `{reflect (B \/ ~A) bona} : reflect (A -> B) bona | 15. exact _. Qed.
+Global Instance reflect_impl {A B a b} `{reflect A a, reflect B b} : reflect (A -> B) (implb a b) | 10. exact _. Qed.
+Global Instance reflect_iff {A B a b} `{reflect A a, reflect B b} : reflect (A <-> B) (Bool.eqb a b) | 10. exact _. Qed.
+Lemma reflect_not {A a} `{reflect A a} : reflect (~A) (negb a).
+Proof. exact _. Qed.
+
+(** Disallow infinite loops of reflect_not *)
+Hint Extern 0 (reflect (~?A) _) => eapply (@reflect_not A) : typeclass_instances.
+
+Global Instance reflect_eq_unit : reflect_rel (@eq unit) (fun _ _ => true) | 10. exact _. Qed.
+Global Instance reflect_eq_bool : reflect_rel (@eq bool) Bool.eqb | 10. exact _. Qed.
+Global Instance reflect_eq_Empty_set : reflect_rel (@eq Empty_set) (fun _ _ => true) | 10. exact _. Qed.
+Global Instance reflect_eq_prod {A B eqA eqB} `{reflect_rel (@eq A) eqA, reflect_rel (@eq B) eqB} : reflect_rel (@eq (A * B)) (prod_beq A B eqA eqB) | 10. exact _. Qed.
+Global Instance reflect_eq_option {A eqA} `{reflect_rel (@eq A) eqA} : reflect_rel (@eq (option A)) (option_beq eqA) | 10. exact _. Qed.
+Global Instance reflect_eq_list {A eqA} `{reflect_rel (@eq A) eqA} : reflect_rel (@eq (list A)) (list_beq A eqA) | 10. exact _. Qed.
+Global Instance reflect_eq_list_nil_r {A eqA} {ls} : reflect (ls = @nil A) (list_beq A eqA ls (@nil A)) | 10.
+Proof. destruct ls; [ left; reflexivity | right; abstract congruence ]. Qed.
+Global Instance reflect_eq_list_nil_l {A eqA} {ls} : reflect (@nil A = ls) (list_beq A eqA (@nil A) ls) | 10.
+Proof. destruct ls; [ left; reflexivity | right; abstract congruence ]. Qed.
+Global Instance reflect_eq_sum {A B eqA eqB} `{reflect_rel (@eq A) eqA, reflect_rel (@eq B) eqB} : reflect_rel (@eq (A + B)) (sum_beq A B eqA eqB) | 10. exact _. Qed.
+Global Instance reflect_eq_sigT_hprop {A P eqA} `{reflect_rel (@eq A) eqA, forall a : A, IsHProp (P a)} : reflect_rel (@eq (@sigT A P)) (sigT_beq eqA (fun _ _ _ _ => true)) | 10. exact _. Qed.
+Global Instance reflect_eq_sig_hprop {A eqA} {P : A -> Prop} `{reflect_rel (@eq A) eqA, forall a : A, IsHProp (P a)} : reflect_rel (@eq (@sig A P)) (sig_beq eqA (fun _ _ _ _ => true)) | 10. exact _. Qed.
+Global Instance reflect_eq_comparison : reflect_rel (@eq comparison) comparison_beq | 10. exact _. Qed.
+
+Module Nat.
+  Definition geb_spec0 : reflect_rel ge (fun x y => Nat.leb y x) := fun _ _ => Nat.leb_spec0 _ _.
+  Definition gtb_spec0 : reflect_rel gt (fun x y => Nat.ltb y x) := fun _ _ => Nat.ltb_spec0 _ _.
+End Nat.
+Global Existing Instance Nat.eqb_spec | 10.
+Global Existing Instances Nat.leb_spec0 Nat.ltb_spec0 Nat.geb_spec0 Nat.gtb_spec0.
+
+Module N.
+  Lemma geb_spec0 : reflect_rel N.ge (fun x y => N.leb y x).
+  Proof. intros x y; generalize (N.leb_spec0 y x); intro H; destruct H; constructor; rewrite N.ge_le_iff; assumption. Qed.
+  Lemma gtb_spec0 : reflect_rel N.gt (fun x y => N.ltb y x).
+  Proof. intros x y; generalize (N.ltb_spec0 y x); intro H; destruct H; constructor; rewrite N.gt_lt_iff; assumption. Qed.
+End N.
+Global Existing Instance N.eqb_spec | 10.
+Global Existing Instances N.leb_spec0 N.ltb_spec0 N.geb_spec0 N.gtb_spec0.
+
+Module Z.
+  Lemma geb_spec0 : reflect_rel Z.ge Z.geb.
+  Proof. intros x y; generalize (Z.leb_spec0 y x); rewrite Z.geb_leb; intro H; destruct H; constructor; rewrite Z.ge_le_iff; assumption. Qed.
+  Lemma gtb_spec0 : reflect_rel Z.gt Z.gtb.
+  Proof. intros x y; generalize (Z.ltb_spec0 y x); rewrite Z.gtb_ltb; intro H; destruct H; constructor; rewrite Z.gt_lt_iff; assumption. Qed.
+End Z.
+Global Existing Instance Z.eqb_spec | 10.
+Global Existing Instances Z.leb_spec0 Z.ltb_spec0 Z.geb_spec0 Z.gtb_spec0.
+
+Module Pos.
+  Lemma geb_spec0 : reflect_rel Pos.ge (fun x y => Pos.leb y x).
+  Proof. intros x y; generalize (Pos.leb_spec0 y x); intro H; destruct H; constructor; rewrite Pos.ge_le_iff; assumption. Qed.
+  Lemma gtb_spec0 : reflect_rel Pos.gt (fun x y => Pos.ltb y x).
+  Proof. intros x y; generalize (Pos.ltb_spec0 y x); intro H; destruct H; constructor; rewrite Pos.gt_lt_iff; assumption. Qed.
+End Pos.
+Global Existing Instance Pos.eqb_spec | 10.
+Global Existing Instances Pos.leb_spec0 Pos.ltb_spec0 Pos.geb_spec0 Pos.gtb_spec0.
+
+Global Instance reflect_Forall {A P Pb} {HD : forall x : A, reflect (P x) (Pb x)} {ls}
+  : reflect (List.Forall P ls) (List.forallb Pb ls) | 10.
+Proof.
+  induction ls as [|x xs IHxs]; cbn [List.forallb]; [ left | destruct (HD x), IHxs; [ left | right.. ] ];
+    [ constructor; assumption | constructor; assumption | intro Hn.. ];
+    clear HD;
+    try abstract (inversion Hn; subst; tauto).
+Qed.
+Global Instance reflect_Exists {A P Pb} {HD : forall x : A, reflect (P x) (Pb x)} {ls}
+  : reflect (List.Exists P ls) (List.existsb Pb ls) | 10.
+Proof.
+  induction ls as [|x xs IHxs]; cbn [List.existsb]; [ right | destruct (HD x), IHxs; [ left.. | right ] ];
+    [ intro Hn | constructor; assumption.. | intro Hn ];
+    clear HD;
+    try abstract (inversion Hn; subst; tauto).
+Qed.
+
+Global Instance reflect_match_pair {A B} {P : A -> B -> Prop} {Pb : A -> B -> bool} {x : A * B}
+       {HD : reflect (P (fst x) (snd x)) (Pb (fst x) (snd x))}
+  : reflect (let '(a, b) := x in P a b) (let '(a, b) := x in Pb a b) | 1.
+Proof. edestruct (_ : _ * _); assumption. Qed.
+
+Global Instance reflect_if_bool {x : bool} {A B a b} {HA : reflect A a} {HB : reflect B b}
+  : reflect (if x then A else B) (if x then a else b) | 10
+  := if x return reflect (if x then A else B) (if x then a else b)
+     then HA
+     else HB.
+
+Global Instance reflect_ex_forall_not : forall T (P:T->Prop) (exPb:bool) {d:reflect (exists b, P b) exPb}, reflect (forall b, ~ P b) (negb exPb).
+Proof.
+  intros T P exPb d; destruct d; constructor; firstorder.
+Qed.
+
+Global Polymorphic Instance reflect_Proper_iff
+  : Proper (iff ==> eq ==> iffT) reflect | 10.
+Proof.
+  intros A B H b b' ?; subst b'; split; intro H'; destruct H, H'; constructor; auto.
+Qed.
+
+Global Polymorphic Instance reflect_Proper_arrow
+  : Proper (iff ==> eq ==> arrow) reflect | 10.
+Proof.
+  repeat intro; eapply reflect_Proper_iff; try eassumption; easy.
+Qed.
+
+Global Polymorphic Instance reflect_Proper_flip_arrow
+  : Proper (iff ==> eq ==> flip arrow) reflect | 10.
+Proof.
+  repeat intro; eapply reflect_Proper_iff; try eassumption; easy.
+Qed.
+
+Lemma reflect_bool : forall {P b} {Preflect:reflect P b}, b = true -> P.
+Proof. intros P b Preflect; destruct Preflect; solve [ auto | discriminate ]. Qed.
+
+Ltac vm_reflect_no_check := apply reflect_bool; vm_cast_no_check (eq_refl true).
+Ltac lazy_reflect_no_check := apply reflect_bool; exact_no_check (eq_refl true).
+
+Ltac vm_reflect := abstract vm_reflect_no_check.
+Ltac lazy_reflect := abstract lazy_reflect_no_check.
